Semantic/CoreCapybara.lean
@@ -12,8 +12,6 @@ import Semantic.CoreCapybara.Denotation
 
 import Semantic.CoreCapybara.Fundamental
 
-import Semantic.CoreCapybara.Gaps
-
 import Semantic.CoreCapybara.Safety
 
 import Semantic.CoreCapybara.Semantics.Standardization
